```Haskell
class Monoid m where
  mempty :: m
  mappend :: m -> m -> m
```
```kotlin:ank:silent
interface Monoid<A> {
  fun empty(): A
  fun combine(a: A, b: A): A
}
```
................
```Haskell
instance Monoid [a] where
  mempty = []
  mappend = (++)
```
```kotlin
import arrow.higherkind
import arrow.typeclasses.Monoid

operator fun <A> FreeMonoid<A>.plus(b: FreeMonoid<A>) = FreeMonoid(this.terms + b.terms)

@higherkind
class FreeMonoid<S>(val terms: List<S>): FreeMonoidOf<S> {

    fun <A> run (f: (S) -> A) = {
       M:Monoid<A> -> M.combineAll(terms.map(f))
    }

    companion object {
        fun <A> mempty(): FreeMonoid<A> = FreeMonoid(listOf())
        fun <A> just(a: A): FreeMonoid<A> = FreeMonoid(listOf(a))
    }
}

fun <A> freeMonoidMonoid(): Monoid<FreeMonoid<A>>  = object: Monoid<FreeMonoid<A>> {
    override fun FreeMonoid<A>.combine(y: FreeMonoid<A>): FreeMonoid<A> =
        FreeMonoid(this.terms + y.terms)

    override fun empty(): FreeMonoid<A> = FreeMonoid.mempty()
}
```
................
```Haskell
2 * 3 = 6
[2] ++ [3] = [2, 3] // not the same as [6]
```
```kotlin
2 * 3 == 6
listOf(2) + listOf(3) == listOf(2, 3) // not the same as listOf(6)
```

................
```Haskell
h (a * b) = h a * h b
```
```kotlin
h(a * b) == h(a) * h(b)
```

................
```Haskell
[2] ++ [3] = [2, 3]
```
```kotlin
listOf(2) + listOf(3) == listOf(2, 3)
```

................
```Haskell
2 * 3 = 6
```
```kotlin
2 * 3 == 6
```
................
```Haskell
p :: x -> U m
```
```kotlin
val p : (X) -> Kind<U, M>
```

................
```Haskell
q :: x -> U n
```
```kotlin
val q: (X) -> Kind<U, N>
```

................
```Haskell
h :: m -> n
```
```kotlin
val h: (M) -> N
```

................
```Haskell
q = U(h) . p
```
```kotlin
val q = uh compose p
```
