```Haskell
a -> m b
```
```scala
A => M[B]
```
................
```Haskell
w a -> b
```
```scala
W[A] => B
```
................
```Haskell
(=>=) :: (w a -> b) -> (w b -> c) -> (w a -> c)
```
```scala
def =>=[A, B, C](w1: W[A] => B)(w2: W[B] => C): W[A] => C

```
................
```Haskell
extract :: w a -> a
```
```scala
def extract[A](wa: W[A]): A
```
................
```Haskell
class Functor w => Comonad w where
    (=>=) :: (w a -> b) -> (w b -> c) -> (w a -> c)
    extract :: w a -> a
```
```scala
trait Comonad[W[_]] extends Functor[W] {
  def =>=[A, B, C](w1: W[A] => B)(w2: W[B] => C): W[A] => C
  def extract[A](wa: W[A]): A
}
```
................
```Haskell
(a, e) -> b
```
```scala
((A, E)) => B
```
................
```Haskell
a -> (e -> b)
```
```scala
A => (E => B)
```
................
```Haskell
data Product e a = Prod e a deriving Functor
```
```scala
case class Product[E, A](run: (E, A))

// implicit def productFunctor = ...
```
................
```Haskell
(=>=) :: (Product e a -> b) -> (Product e b -> c) -> (Product e a -> c)
f =>= g = \(Prod e a) -> let b = f (Prod e a)
                          c = g (Prod e b) 
                      in c
```
```scala
def =>=[E, A, B, C]: (Product[E, A] => B) => (Product[E, B] => C) =>
    (Product[E, A] => C) = f => g => {
  case Product((e, a)) =>
    val b = f(Product((e, a)))
    val c = g(Product((e, b)))
    c
  }

```
................
```Haskell
extract (Prod e a) = a
```
```scala
def extract[E, A]: Product[E, A] => A = {
  case Product((e, a)) => a
}
```
................
```Haskell
(=>=) :: (w a -> b) -> (w b -> c) -> (w a -> c)
f =>= g = g ... 
```
```scala
def =>=[W[_], A, B, C]: (W[A] => B) => (W[B] => C) => (W[A] => C) =
  f => g => g ...
```
................
```Haskell
extend :: (w a -> b) -> w a -> w b
```
```scala
def extend[W[_], A, B]: (W[A] => B) => W[A] => W[B]
```
................
```Haskell
f =>= g = g . extend f
```
```scala
def =>=[W[_], A, B, C]: (W[A] => B) => (W[B] => C) => (W[A] => C) =
  f => g => g compose extend(f)
```
................
```Haskell
duplicate :: w a -> w (w a)
```
```scala
def duplicate[W[_], A]: W[A] => W[W[A]]
```
................
```Haskell
class Functor w => Comonad w where
    extract :: w a -> a
    duplicate :: w a -> w (w a)
    duplicate = extend id
    extend :: (w a -> b) -> w a -> w b
    extend f = fmap f . duplicate
```
```scala
trait Comonad[W[_]] extends Functor[W] {
  def extract[A](wa: W[A]): A

  def duplicate[A](wa: W[A]): W[W[A]] =
    extend(identity[W[A]])(wa)

  def extend[A, B](f: W[A] => B)(wa: W[A]): W[B] =
    (fmap(f) _ compose duplicate)(wa)
}
```
................
```Haskell
data Stream a = Cons a (Stream a)
```
```scala
case class Stream[A](h: () => A, t: () => Stream[A])
```
................
```Haskell
instance Functor Stream where
    fmap f (Cons a as) = Cons (f a) (fmap f as)
```
```scala
implicit val streamFunctor = new Functor[Stream] {
  def fmap[A, B](f: A => B)(fa: Stream[A]): Stream[B] = fa match {
    case Stream(a, as) =>
      Stream(() => f(a()), () => fmap(f)(as()))
  }
}
```
................
```Haskell
extract (Cons a _) = a
```
```scala
def extract[A](wa: Stream[A]): A = wa match {
  case Stream(a, _) => a()
}
```
................
```Haskell
duplicate (Cons a as) = Cons (Cons a as) (duplicate as)
```
```scala
def duplicateS[A](wa: Stream[A]): Stream[Stream[A]] = wa match {
  case s @ Stream(a, as) =>
    Stream(() => s, () => duplicateS(as()))
}
```
................
```Haskell
instance Comonad Stream where
    extract (Cons a _) = a 
    duplicate (Cons a as) = Cons (Cons a as) (duplicate as)
```
```scala
implicit val streamComonad = new Comonad[Stream] {
  def extract[A](wa: Stream[A]): A =
    wa match {
      case Stream(a, _) => a()
    }

  def duplicate[A](wa: Stream[A]): Stream[Stream[A]] = wa match {
    case s @ Stream(a, as) =>
      Stream(() => s, () => duplicate(as()))
  }
}
```
................
```Haskell
tail :: Stream a -> Stream a
tail (Cons a as) = as
```
```scala
def tail[A]: Stream[A] => Stream[A] = {
  case Stream(a, as) => as()
}
```
................
```Haskell
sumS :: Num a => Int -> Stream a -> a
sumS n (Cons a as) = if n <= 0 then 0 else a + sumS (n - 1) as
```
```scala
def sumS[A](n: Int)(stm: Stream[A])(implicit numeric: Numeric[A]): A =
  stm match {
    case Stream(a, as) =>
      import numeric._
      if (n <= 0) zero else a() + sumS(n - 1)(as())
  }
```
................
```Haskell
average :: Fractional a => Int -> Stream a -> a
average n stm = (sumS n stm) / (fromIntegral n)
```
```scala
def average[A](n: Int)
    (implicit fractional: Fractional[A]): Stream[A] => A = stm => {
  import fractional._
  sumS(n)(stm) / fromInt(n)
}
```
................
```Haskell
movingAvg :: Fractional a => Int -> Stream a -> Stream a
movingAvg n = extend (average n)
```
```scala
def movingAvg[A](n: Int)(stm: Stream[A])
    (implicit fractional: Fractional[A]): Stream[A] =
  streamComonad.
    extend(average(n)(fractional))(stm)
```
................
```Haskell
class Comonoid m where
    split :: m -> (m, m)
    destroy :: m -> ()
```
```scala
trait Comonoid[M] {
  def split(x: M): (M, M)
  def destroy(x: M): Unit
}
```
................
```Haskell
destroy _ = ()
```
```scala
def destroy(x: M): Unit = ()
```
................
```Haskell
split x = (f x, g x)
```
```scala
def split(x: M): (M, M) = (f(x), g(x))
```
................
```Haskell
lambda . bimap destroy id . split = id
rho . bimap id destroy . split = id
```
```scala
(lambda compose bimap(destroy)(identity[M]))
  .compose(split) == identity[M]

(rho compose bimap(identity[M])(destroy))
  .compose(split) == identity[M]
```
................
```Haskell
lambda (bimap destroy id (split x))
= lambda (bimap destroy id (f x, g x))
= lambda ((), g x)
= g x
```
```scala
lambda(bimap(destroy)(identity[M])(split(x))) ==
  lambda(bimap(destroy)(identity[M])((f(x), g(x)))) ==
  lambda(((), g(x))) ==
  g(x)
```
................
```Haskell
split x = (x, x)
```
```scala
def split(x: M): (M, M) = (x, x)
```
................
```Haskell
data Store s a = Store (s -> a) s
```
```scala
case class Store[S, A](run: S => A, s: S)
```
................
```Haskell
counit (Prod (Reader f) s)) = f s
```
```scala
def counit[S, A](a: Product[S, Reader[S, A]]): A = a match {
  case Product((Reader(f), s)) => f(s)
}
```
................
```Haskell
extract (Store f s) = f s
```
```scala
def extract[A](wa: Store[S, A]): A = wa match {
  case Store(f, s) => f(s)
}
```
................
```Haskell
unit :: a -> Reader s (Product a s)
unit a = Reader (\s -> Prod a s)
```
```scala
def unit[S, A](a: A): Reader[S, Product[S, A]] =
  Reader(s => Product((a, s)))
```
................
```Haskell
Store f :: s -> Store f s
```
```scala
object Store {
  def apply[S, A](run: S => A): S => Store[S, A] =
    s => new Store(run, s)
}
```
................
```Haskell
duplicate (Store f s) = Store (Store f) s
```
```scala
def duplicate[A](wa: Store[S, A]): Store[S, Store[S, A]] = wa match {
  case Store(f, s) => Store(Store(f), s)
}
```
................
```Haskell
instance Comonad (Store s) where
    extract (Store f s) = f s
    duplicate (Store f s) = Store (Store f) s
```
```scala
implicit def storeComonad[S] = new Comonad[Store[S, ?]] {
  def extract[A](wa: Store[S, A]): A = wa match {
    case Store(f, s) => f(s)
  }

  override def duplicate[A](wa: Store[S, A]): Store[S, Store[S, A]] =
    wa match {
      case Store(f, s) => Store(Store(f), s)
    }
}
```
................
```Haskell
a -> Store s a
```
```scala
A => Store[S, A]
```
................
```Haskell
set :: a -> s -> a
get :: a -> s
```
```scala
def set[A, S]: A => S => A
def get[A, S]: A => S
```
................
